src/proof/algebra/mono_gset.v
@@ -61,7 +61,7 @@ Definition own_auth γ s : iProp Σ :=
 Definition own_frag γ a : iProp Σ :=
   own γ (◯ {[a]}).
 
-Lemma frag_elem_of_auth γ s a:
+Lemma frag_elem_of_auth {γ s} a:
 own_auth γ s -∗ own_frag γ a -∗ ⌜ a ∈ s ⌝.
 Proof.
   iIntros "Hauth Hfrag".
@@ -71,7 +71,7 @@ Proof.
   done.
 Qed.
 
-Lemma insert_vs γ s a:
+Lemma insert_vs {γ s} a:
 own_auth γ s ==∗ own_auth γ (s ∪ {[a]}) ∗ own_frag γ a.
 Proof.
   iIntros "Hauth".
