src/proof/reflect_init.v
@@ -1,0 +1,10 @@
+Require Export New.generatedproof.reflect.
+
+
+Section proof.
+Context `{hG: heapGS Σ} `{!ffi_semantics _ _} {go_ctx: GoContext}.
+
+#[global] Instance : IsPkgInit code.reflect.reflect := define_is_pkg_init True%I.
+#[global] Instance : GetIsPkgInitWf code.reflect.reflect := build_get_is_pkg_init_wf.
+
+End proof.
